Definition and spec for point add fn

src/Bedrock/End2End/X25519/MontgomeryLadder.v
@@ -35,6 +35,30 @@ Definition mul_and_add := func! (o, x, y) {
   fe25519_add(o, o, y)
 }.
 
+(* Better way to represent points in Bedrock2? *)
+Definition add_precomputed := func! (ox, oy, oz, ot, X1, Y1, Z1, T1, ypx2, ymx2, xy2d2) {
+  stackalloc 40 as YpX1;
+  fe25519_add(YpX1, Y1, X1);
+  stackalloc 40 as YmX1;
+  fe25519_sub(YmX1, Y1, X1);
+  stackalloc 40 as A;
+  fe25519_mul(A, YpX1, ypx2);
+  stackalloc 40 as B;
+  fe25519_mul(B, YmX1, ymx2);
+  stackalloc 40 as C;
+  fe25519_mul(C, xy2d2, T1);
+  stackalloc 40 as D;
+  fe25519_add(D, Z1, Z1);
+  fe25519_sub(ox, A, B);
+  fe25519_add(oy, A, B);
+  fe25519_add(oz, D, C);
+  fe25519_sub(ot, D, C);
+  fe25519_mul(ox, ox, ot);
+  fe25519_mul(oy, oy, oz);
+  fe25519_mul(oz, ot, oz);
+  fe25519_mul(ot, ox, oy)
+}.
+
 Require Import bedrock2.FE310CSemantics bedrock2.Semantics .
 Require Import bedrock2.WeakestPrecondition bedrock2.ProgramLogic.
 Require Import coqutil.Word.Interface coqutil.Word.Bitwidth.
@@ -58,7 +82,7 @@ Local Notation "xs $@ a" := (Array.array ptsto (word.of_Z 1) a xs) (at level 10,
 Local Notation FElem := (FElem(FieldRepresentation:=frep25519)).
 Local Notation bounded_by := (bounded_by(FieldRepresentation:=frep25519)).
 Local Notation word := (Naive.word 32).
-Local Notation felem := (felem(FieldRepresentation:=frep25519)). 
+Local Notation felem := (felem(FieldRepresentation:=frep25519)).
 
 Global Instance spec_of_square_and_add : spec_of "square_and_add" :=
   fnspec! "square_and_add" (out xk yk: word) / (o x y : felem) (R : _ -> Prop),
@@ -84,9 +108,36 @@ Global Instance spec_of_mul_and_add : spec_of "mul_and_add" :=
         /\ bounded_by loose_bounds o'
         /\ m' =* (FElem xk x) * (FElem yk y) * (FElem out o') * R }.
 
+Require Import Curves.Edwards.XYZT.Precomputed. (* Move elsewhere *)
+
+Global Instance spec_of_add_precomputed : spec_of "add_precomputed" :=
+  fnspec! "add_precomputed"
+    (oxK oyK ozK otK X1K Y1K Z1K T1K ypx2K ymx2K xy2d2K : word) /
+    (ox oy oz ot X1 Y1 Z1 T1 ypx2 ymx2 xy2d2 : felem) (R : _ -> Prop),
+  { requires t m :=
+      bounded_by tight_bounds X1 /\
+      bounded_by tight_bounds Y1 /\
+      bounded_by tight_bounds Z1 /\ (* Could be loose if switch to mul *)
+      bounded_by loose_bounds T1 /\
+      bounded_by loose_bounds ypx2 /\
+      bounded_by loose_bounds ymx2 /\
+      bounded_by loose_bounds xy2d2 /\
+      m =* (FElem X1K X1) * (FElem Y1K Y1) * (FElem Z1K Z1) * (FElem T1K T1) * (FElem ypx2K ypx2) * (FElem ymx2K ymx2) * (FElem xy2d2K xy2d2) * (FElem oxK ox) * (FElem oyK oy) * (FElem ozK oz) * (FElem otK ot) * R;
+    ensures t' m' :=
+      t = t' /\
+      exists ox' oy' oz' ot',
+        (* Need to specify implicit parameters? *)
+        ((feval ox'), (feval oy'), (feval oz'), (feval ot')) = (@m1add_precomputed_coordinates (F M_pos) (F.add) (F.sub) (F.mul) ((feval X1), (feval Y1), (feval Z1), (feval T1)) ((feval ypx2), (feval ymx2), (feval xy2d2))) /\
+        bounded_by loose_bounds ox' /\
+        bounded_by loose_bounds oy' /\
+        bounded_by loose_bounds oz' /\
+        bounded_by loose_bounds ot' /\
+        m' =* (FElem X1K X1) * (FElem Y1K Y1) * (FElem Z1K Z1) * (FElem T1K T1) * (FElem ypx2K ypx2) * (FElem ymx2K ymx2) * (FElem xy2d2K xy2d2) * (FElem oxK ox') * (FElem oyK oy') * (FElem ozK oz') * (FElem otK ot') * R }.
+
 Local Instance spec_of_fe25519_square : spec_of "fe25519_square" := Field.spec_of_UnOp un_square.
 Local Instance spec_of_fe25519_mul : spec_of "fe25519_mul" := Field.spec_of_BinOp bin_mul.
 Local Instance spec_of_fe25519_add : spec_of "fe25519_add" := Field.spec_of_BinOp bin_add.
+Local Instance spec_of_fe25519_sub : spec_of "fe25519_sub" := Field.spec_of_BinOp bin_sub.
 
 Import WeakestPrecondition.
 
